Updating to use the native string type

src/AbstractedTypes.v
@@ -1,16 +1,17 @@
 (* Abstract (Admitted) definition of a general type for 
     Identifiers and associated abstract values/operations *)
 
-Require Export ResultT EqClass StringT.
+Require Export ResultT EqClass.
+Require Import String.
 
 (* Abstract type reserved for Identifiers *)
 Definition ID_Type : Set. Admitted.
 
-Definition ID_Type_to_stringT (id:ID_Type) : StringT. Admitted.
-Definition stringT_to_ID_Type (s:StringT) : ResultT ID_Type StringT. Admitted.
+Definition ID_Type_to_string (id:ID_Type) : string. Admitted.
+Definition string_to_ID_Type (s:string) : ResultT ID_Type string. Admitted.
 
-Axiom canonical_string_id_type : forall (s : StringT) (i : ID_Type),
-  ID_Type_to_stringT i = s <-> (stringT_to_ID_Type s = resultC i).
+Axiom canonical_string_id_type : forall (s : string) (i : ID_Type),
+  ID_Type_to_string i = s <-> (string_to_ID_Type s = resultC i).
 
 (* Assumed equality for identifiers *)
 Global Instance Eq_Class_ID_Type : EqClass ID_Type. Admitted.
