src/ErrorStringConstants.v
@@ -2,70 +2,70 @@
     Once instantiated, these should provide descriptive error messages for 
     dynamic error cases in Coq-extracted code. *)
 
-Require Import StringT.
+Require Import String.
 
-Definition empty_string : StringT. Admitted.
+Definition empty_string : string. Admitted.
 
-Definition errStr_amNonce : StringT. Admitted.
+Definition errStr_amNonce : string. Admitted.
 
-Definition errStr_peel_bs_am : StringT. Admitted.
+Definition errStr_peel_bs_am : string. Admitted.
 
-Definition errStr_peel_n_am : StringT. Admitted.
+Definition errStr_peel_n_am : string. Admitted.
 
-Definition errStr_requester_bound : StringT. Admitted.
+Definition errStr_requester_bound : string. Admitted.
 
-Definition errStr_disclosePolicy : StringT. Admitted.
+Definition errStr_disclosePolicy : string. Admitted.
 
-Definition errStr_app_auth_tok : StringT. Admitted.
+Definition errStr_app_auth_tok : string. Admitted.
 
-Definition errStr_dispatch_error : StringT. Admitted.
+Definition errStr_dispatch_error : string. Admitted.
 
-Definition errStr_cvm_error : StringT. Admitted.
+Definition errStr_cvm_error : string. Admitted.
 
-Definition errStr_decryption_prim : StringT. Admitted.
+Definition errStr_decryption_prim : string. Admitted.
 
-Definition errStr_et_size : StringT. Admitted.
+Definition errStr_et_size : string. Admitted.
 
-Definition errStr_lib_supports_man_check : StringT. Admitted.
+Definition errStr_lib_supports_man_check : string. Admitted.
 
-Definition errStr_lib_supports_man_app_check : StringT. Admitted.
+Definition errStr_lib_supports_man_app_check : string. Admitted.
 
 (* Evidence Bundling Errors *)
-Definition errStr_empty_raw_ev : StringT. Admitted.
+Definition errStr_empty_raw_ev : string. Admitted.
 
-Definition errStr_raw_evidence_too_long : StringT. Admitted.
+Definition errStr_raw_evidence_too_long : string. Admitted.
 
-Definition errStr_raw_evidence_wrong_length_comp : StringT. Admitted.
+Definition errStr_raw_evidence_wrong_length_comp : string. Admitted.
 
 (* JSON Interface Error String *)
-Definition errStr_remote_am_failure : StringT. Admitted.
+Definition errStr_remote_am_failure : string. Admitted.
 
-Definition errStr_incorrect_resp_type : StringT. Admitted.
+Definition errStr_incorrect_resp_type : string. Admitted.
 
-Definition errStr_json_parsing : StringT. Admitted.
+Definition errStr_json_parsing : string. Admitted.
 
-Definition errStr_invalid_request_type : StringT. Admitted.
+Definition errStr_invalid_request_type : string. Admitted.
 
-Definition errStr_negotiation_not_implemented : StringT. Admitted.
+Definition errStr_negotiation_not_implemented : string. Admitted.
 
 (* Run CVM Error Strings *)
-Definition errStr_run_cvm_at_error_dynamic : StringT. Admitted.
+Definition errStr_run_cvm_at_error_dynamic : string. Admitted.
 
-Definition errStr_run_cvm_at_error_static : StringT. Admitted.
+Definition errStr_run_cvm_at_error_static : string. Admitted.
 
-Definition errStr_run_cvm_dispatch_unavailable : StringT. Admitted.
+Definition errStr_run_cvm_dispatch_unavailable : string. Admitted.
 
 (* JSON Converter Strings *)
-Definition errStr_json_to_manifest_set : StringT. Admitted.
+Definition errStr_json_to_manifest_set : string. Admitted.
 
-Definition errStr_json_to_map : StringT. Admitted.
+Definition errStr_json_to_map : string. Admitted.
 
-Definition errStr_json_to_id_type : StringT. Admitted.
+Definition errStr_json_to_id_type : string. Admitted.
 
-Definition errStr_json_to_manifest : StringT. Admitted.
+Definition errStr_json_to_manifest : string. Admitted.
 
-Definition errStr_json_to_ASP_Locator : StringT. Admitted.
+Definition errStr_json_to_ASP_Locator : string. Admitted.
 
-Definition errStr_json_to_am_lib : StringT. Admitted.
+Definition errStr_json_to_am_lib : string. Admitted.
 
-Definition errStr_json_to_pair : StringT. Admitted.
+Definition errStr_json_to_pair : string. Admitted.
