src/JSON_Type.v
@@ -1,8 +1,8 @@
-Require Import StringT Maps.
+Require Import String Maps.
 
 Inductive JSON : Type :=
-| JSON_Object : MapC StringT JSON -> JSON
+| JSON_Object : MapC string JSON -> JSON
 | JSON_Array : list JSON -> JSON
-| JSON_String : StringT -> JSON
+| JSON_String : string -> JSON
 | JSON_Boolean : bool -> JSON
 | JSON_Null : JSON.
