src/CvmJson_Interfaces.v
@@ -3,7 +3,7 @@
     
     At the moment, these are too low-level to represent faithfully in the Coq development.   *)
 
-Require Import Term_Defs_Core Term_Defs StringT List JSON Interface_Types ResultT ErrorStringConstants Term_Defs_Admits BS.
+Require Import Term_Defs_Core Term_Defs String List JSON Interface_Types ResultT ErrorStringConstants Term_Defs_Admits BS.
 Export Interface_Types JSON.
 Import ListNotations ResultNotation.
 
@@ -12,17 +12,17 @@ Definition ProtocolRunRequest_to_JSON (req: ProtocolRunRequest): JSON :=
   JSON_Object 
     [(STR_TYPE, (JSON_String STR_REQUEST));
     (STR_ACTION, (JSON_String STR_RUN));
-    (STR_REQ_PLC, (JSON_String (Plc_to_stringT (prreq_req_plc req))));
-    (STR_TERM, (JSON_String (Term_to_stringT (prreq_term req)))); 
-    (STR_EV, (JSON_String (RawEv_to_stringT (prreq_ev req))))].
+    (STR_REQ_PLC, (JSON_String (Plc_to_string (prreq_req_plc req))));
+    (STR_TERM, (JSON_String (Term_to_string (prreq_term req)))); 
+    (STR_EV, (JSON_String (RawEv_to_string (prreq_ev req))))].
 
-Definition JSON_to_ProtocolRunRequest (req : JSON): ResultT ProtocolRunRequest StringT :=
-  temp_term <- JSON_get_stringT STR_TERM req ;;
-  temp_req_plc <- JSON_get_stringT STR_REQ_PLC req ;;
-  temp_ev <- JSON_get_stringT STR_EV req ;;
-  term <- stringT_to_Term temp_term ;;
-  req_plc <- stringT_to_Plc temp_req_plc ;;
-  ev <- stringT_to_RawEv temp_ev ;;
+Definition JSON_to_ProtocolRunRequest (req : JSON): ResultT ProtocolRunRequest string :=
+  temp_term <- JSON_get_string STR_TERM req ;;
+  temp_req_plc <- JSON_get_string STR_REQ_PLC req ;;
+  temp_ev <- JSON_get_string STR_EV req ;;
+  term <- string_to_Term temp_term ;;
+  req_plc <- string_to_Plc temp_req_plc ;;
+  ev <- string_to_RawEv temp_ev ;;
   resultC (mkPRReq term req_plc ev).
 
 Definition ProtocolRunResponse_to_JSON (resp: ProtocolRunResponse): JSON :=
@@ -30,12 +30,12 @@ Definition ProtocolRunResponse_to_JSON (resp: ProtocolRunResponse): JSON :=
     [(STR_TYPE, (JSON_String STR_RESPONSE));
     (STR_ACTION, (JSON_String STR_RUN));
     (STR_SUCCESS, (JSON_Boolean (prresp_success resp)));
-    (STR_PAYLOAD, (JSON_String (RawEv_to_stringT (prresp_ev resp))))].
+    (STR_PAYLOAD, (JSON_String (RawEv_to_string (prresp_ev resp))))].
 
-Definition JSON_to_ProtocolRunResponse (resp : JSON): ResultT ProtocolRunResponse StringT :=
+Definition JSON_to_ProtocolRunResponse (resp : JSON): ResultT ProtocolRunResponse string :=
   temp_success <- JSON_get_bool STR_SUCCESS resp ;;
-  temp_ev <- JSON_get_stringT STR_PAYLOAD resp ;;
-  ev <- stringT_to_RawEv temp_ev ;;
+  temp_ev <- JSON_get_string STR_PAYLOAD resp ;;
+  ev <- string_to_RawEv temp_ev ;;
   resultC (mkPRResp temp_success ev).
 
 (* Protocol Negotiate Section *)
@@ -43,12 +43,12 @@ Definition ProtocolNegotiateRequest_to_JSON (req: ProtocolNegotiateRequest): JSO
   JSON_Object 
     [(STR_TYPE, (JSON_String STR_REQUEST));
     (STR_ACTION, (JSON_String STR_NEGOTIATE));
-      (STR_TERM, (JSON_String (Term_to_stringT (pnreq_term req))))].
+      (STR_TERM, (JSON_String (Term_to_string (pnreq_term req))))].
 
 Definition JSON_to_ProtocolNegotiateRequest (req : JSON): 
-    ResultT ProtocolNegotiateRequest StringT :=
-  temp_term <- JSON_get_stringT STR_TERM req ;;
-  term <- stringT_to_Term temp_term ;;
+    ResultT ProtocolNegotiateRequest string :=
+  temp_term <- JSON_get_string STR_TERM req ;;
+  term <- string_to_Term temp_term ;;
   resultC (mkPNReq term).
 
 Definition ProtocolNegotiateResponse_to_JSON (resp: ProtocolNegotiateResponse): JSON :=
@@ -56,13 +56,13 @@ Definition ProtocolNegotiateResponse_to_JSON (resp: ProtocolNegotiateResponse): 
     [(STR_TYPE, (JSON_String STR_RESPONSE));
     (STR_ACTION, (JSON_String STR_NEGOTIATE));
       (STR_SUCCESS, (JSON_Boolean (pnresp_success resp)));
-    (STR_PAYLOAD, (JSON_String (Term_to_stringT (pnresp_term resp))))].
+    (STR_PAYLOAD, (JSON_String (Term_to_string (pnresp_term resp))))].
 
 Definition JSON_to_ProtocolNegotiateResponse (resp : JSON): 
-    ResultT ProtocolNegotiateResponse StringT :=
+    ResultT ProtocolNegotiateResponse string :=
   temp_success <- JSON_get_bool STR_SUCCESS resp ;;
-  temp_term <- JSON_get_stringT STR_PAYLOAD resp ;;
-  term <- stringT_to_Term temp_term ;;
+  temp_term <- JSON_get_string STR_PAYLOAD resp ;;
+  term <- string_to_Term temp_term ;;
   resultC (mkPNResp temp_success term).
 
 (* Protocol Appraise Section *)
@@ -70,21 +70,21 @@ Definition ProtocolAppraiseRequest_to_JSON (req: ProtocolAppraiseRequest): JSON 
   JSON_Object 
     [(STR_TYPE, (JSON_String STR_REQUEST));
     (STR_ACTION, (JSON_String STR_APPRAISE));
-    (STR_TERM, (JSON_String (Term_to_stringT (pareq_term req))));
-    (STR_REQ_PLC, (JSON_String (Plc_to_stringT (pareq_plc req))));
-    (STR_EVIDENCE, (JSON_String (Evidence_to_stringT (pareq_evidence req))));
-    (STR_EV, (JSON_String (RawEv_to_stringT (pareq_ev req))))].
+    (STR_TERM, (JSON_String (Term_to_string (pareq_term req))));
+    (STR_REQ_PLC, (JSON_String (Plc_to_string (pareq_plc req))));
+    (STR_EVIDENCE, (JSON_String (Evidence_to_string (pareq_evidence req))));
+    (STR_EV, (JSON_String (RawEv_to_string (pareq_ev req))))].
 
 Definition JSON_to_ProtocolAppraiseRequest (req : JSON): 
-    ResultT ProtocolAppraiseRequest StringT :=
-  temp_term <- JSON_get_stringT STR_TERM req ;;
-  temp_plc <- JSON_get_stringT STR_REQ_PLC req ;;
-  temp_evidence <- JSON_get_stringT STR_EVIDENCE req ;;
-  temp_ev <- JSON_get_stringT STR_EV req ;;
-  term <- stringT_to_Term temp_term ;;
-  plc <- stringT_to_Plc temp_plc ;;
-  evidence <- stringT_to_Evidence temp_evidence ;;
-  ev <- stringT_to_RawEv temp_ev ;;
+    ResultT ProtocolAppraiseRequest string :=
+  temp_term <- JSON_get_string STR_TERM req ;;
+  temp_plc <- JSON_get_string STR_REQ_PLC req ;;
+  temp_evidence <- JSON_get_string STR_EVIDENCE req ;;
+  temp_ev <- JSON_get_string STR_EV req ;;
+  term <- string_to_Term temp_term ;;
+  plc <- string_to_Plc temp_plc ;;
+  evidence <- string_to_Evidence temp_evidence ;;
+  ev <- string_to_RawEv temp_ev ;;
   resultC (mkPAReq term plc evidence ev).
 
 Definition ProtocolAppraiseResponse_to_JSON (resp: ProtocolAppraiseResponse): JSON :=
@@ -92,13 +92,13 @@ Definition ProtocolAppraiseResponse_to_JSON (resp: ProtocolAppraiseResponse): JS
     [(STR_TYPE, (JSON_String STR_RESPONSE));
     (STR_ACTION, (JSON_String STR_APPRAISE));
     (STR_SUCCESS, (JSON_Boolean (paresp_success resp)));
-    (STR_PAYLOAD, (JSON_String (AppResultC_to_stringT (paresp_result resp))))].
+    (STR_PAYLOAD, (JSON_String (AppResultC_to_string (paresp_result resp))))].
 
 Definition JSON_to_ProtocolAppraiseResponse (resp : JSON): 
-    ResultT ProtocolAppraiseResponse StringT :=
+    ResultT ProtocolAppraiseResponse string :=
   temp_success <- JSON_get_bool STR_SUCCESS resp ;;
-  temp_result <- JSON_get_stringT STR_PAYLOAD resp ;;
-  result <- stringT_to_AppResultC temp_result ;;
+  temp_result <- JSON_get_string STR_PAYLOAD resp ;;
+  result <- string_to_AppResultC temp_result ;;
   resultC (mkPAResp temp_success result).
 
 (* AM Protocol Request Section *)
@@ -110,8 +110,8 @@ Definition AM_Protocol_Request_to_JSON (req: AM_Protocol_Requests): JSON :=
   end.
 
 Definition JSON_to_AM_Protocol_Request (req : JSON): 
-    ResultT AM_Protocol_Requests StringT :=
-  temp_type <- JSON_get_stringT STR_ACTION req ;;
+    ResultT AM_Protocol_Requests string :=
+  temp_type <- JSON_get_string STR_ACTION req ;;
   if (eqb temp_type STR_RUN)
   then (temp_req <- JSON_to_ProtocolRunRequest req ;;
         resultC (Protocol_Run_Request temp_req))
@@ -132,8 +132,8 @@ Definition AM_Protocol_Response_to_JSON (resp: AM_Protocol_Responses): JSON :=
   end.
 
 Definition JSON_to_AM_Protocol_Response (resp : JSON): 
-    ResultT AM_Protocol_Responses StringT :=
-  temp_type <- JSON_get_stringT STR_ACTION resp ;;
+    ResultT AM_Protocol_Responses string :=
+  temp_type <- JSON_get_string STR_ACTION resp ;;
   if (eqb temp_type STR_RUN)
   then (temp_resp <- JSON_to_ProtocolRunResponse resp ;;
         resultC (Protocol_Run_Response temp_resp))
@@ -153,8 +153,8 @@ Definition AM_Protocol_Interface_to_JSON (msg: AM_Protocol_Interface): JSON :=
   end.
 
 Definition JSON_to_AM_Protocol_Interface (msg : JSON): 
-    ResultT AM_Protocol_Interface StringT :=
-  temp_type <- JSON_get_stringT STR_TYPE msg ;;
+    ResultT AM_Protocol_Interface string :=
+  temp_type <- JSON_get_string STR_TYPE msg ;;
   if (eqb temp_type STR_REQUEST)
   then (temp_msg <- JSON_to_AM_Protocol_Request msg ;;
         resultC (AM_Protocol_Request_Interface temp_msg))
@@ -169,23 +169,23 @@ Definition ASPRunRequest_to_JSON (req: ASPRunRequest): JSON :=
   JSON_Object 
     [(STR_TYPE, (JSON_String STR_REQUEST));
     (STR_ACTION, (JSON_String STR_ASP_RUN));
-    (STR_ASP_ID, (JSON_String (ASP_ID_to_stringT (asprreq_asp_id req))));
-    (STR_ASP_ARGS, (JSON_String (ASP_ARGS_to_stringT (asprreq_asp_args req))));
-    (STR_TARG_PLC, (JSON_String (Plc_to_stringT (asprreq_targ_plc req))));
-    (STR_TARG, (JSON_String (TARG_ID_to_stringT (asprreq_targ req))));
-    (STR_EV, (JSON_String (RawEv_to_stringT (asprreq_rawev req))))].
+    (STR_ASP_ID, (JSON_String (ASP_ID_to_string (asprreq_asp_id req))));
+    (STR_ASP_ARGS, (JSON_String (ASP_ARGS_to_string (asprreq_asp_args req))));
+    (STR_TARG_PLC, (JSON_String (Plc_to_string (asprreq_targ_plc req))));
+    (STR_TARG, (JSON_String (TARG_ID_to_string (asprreq_targ req))));
+    (STR_EV, (JSON_String (RawEv_to_string (asprreq_rawev req))))].
 
-Definition JSON_to_ASPRunRequest (req : JSON): ResultT ASPRunRequest StringT :=
-  temp_asp_id <- JSON_get_stringT STR_ASP_ID req ;;
-  temp_asp_args <- JSON_get_stringT STR_ASP_ARGS req ;;
-  temp_targ_plc <- JSON_get_stringT STR_TARG_PLC req ;;
-  temp_targ <- JSON_get_stringT STR_TARG req ;;
-  temp_ev <- JSON_get_stringT STR_EV req ;;
-  asp_id <- stringT_to_ASP_ID temp_asp_id ;;
-  asp_args <- stringT_to_ASP_ARGS temp_asp_args ;;
-  targ_plc <- stringT_to_Plc temp_targ_plc ;;
-  targ <- stringT_to_TARG_ID temp_targ ;;
-  ev <- stringT_to_RawEv temp_ev ;;
+Definition JSON_to_ASPRunRequest (req : JSON): ResultT ASPRunRequest string :=
+  temp_asp_id <- JSON_get_string STR_ASP_ID req ;;
+  temp_asp_args <- JSON_get_string STR_ASP_ARGS req ;;
+  temp_targ_plc <- JSON_get_string STR_TARG_PLC req ;;
+  temp_targ <- JSON_get_string STR_TARG req ;;
+  temp_ev <- JSON_get_string STR_EV req ;;
+  asp_id <- string_to_ASP_ID temp_asp_id ;;
+  asp_args <- string_to_ASP_ARGS temp_asp_args ;;
+  targ_plc <- string_to_Plc temp_targ_plc ;;
+  targ <- string_to_TARG_ID temp_targ ;;
+  ev <- string_to_RawEv temp_ev ;;
   resultC (mkASPRReq asp_id asp_args targ_plc targ ev).
 
 Definition ASPRunResponse_to_JSON (resp: ASPRunResponse): JSON :=
@@ -193,12 +193,12 @@ Definition ASPRunResponse_to_JSON (resp: ASPRunResponse): JSON :=
     [(STR_TYPE, (JSON_String STR_RESPONSE));
     (STR_ACTION, (JSON_String STR_ASP_RUN));
     (STR_SUCCESS, (JSON_Boolean (asprresp_success resp)));
-    (STR_PAYLOAD, (JSON_String (RawEv_to_stringT (asprresp_rawev resp))))].
+    (STR_PAYLOAD, (JSON_String (RawEv_to_string (asprresp_rawev resp))))].
 
-Definition JSON_to_ASPRunResponse (resp : JSON): ResultT ASPRunResponse StringT :=
+Definition JSON_to_ASPRunResponse (resp : JSON): ResultT ASPRunResponse string :=
   temp_success <- JSON_get_bool STR_SUCCESS resp ;;
-  temp_rawev <- JSON_get_stringT STR_PAYLOAD resp ;;
-  rawev <- stringT_to_RawEv temp_rawev ;;
+  temp_rawev <- JSON_get_string STR_PAYLOAD resp ;;
+  rawev <- string_to_RawEv temp_rawev ;;
   resultC (mkASPRResp temp_success rawev).
 
 (* AM ASP Interface Section *)
@@ -210,9 +210,9 @@ Definition AM_ASP_Interface_to_JSON (msg: AM_ASP_Interface): JSON :=
   end.
 
 Definition JSON_to_AM_ASP_Interface (msg : JSON): 
-    ResultT AM_ASP_Interface StringT :=
-  temp_type <- JSON_get_stringT STR_TYPE msg ;;
-  temp_action <- JSON_get_stringT STR_ACTION msg ;;
+    ResultT AM_ASP_Interface string :=
+  temp_type <- JSON_get_string STR_TYPE msg ;;
+  temp_action <- JSON_get_string STR_ACTION msg ;;
   if (eqb temp_type STR_REQUEST)
   then if (eqb temp_action STR_ASP_RUN)
        then (temp_msg <- JSON_to_ASPRunRequest msg ;;
@@ -226,7 +226,7 @@ Definition JSON_to_AM_ASP_Interface (msg : JSON):
   else errC errStr_incorrect_resp_type.
 
 (* Error Response *)
-Definition ErrorResponseJSON (msg: StringT): JSON :=
+Definition ErrorResponseJSON (msg: string): JSON :=
   JSON_Object 
     [(STR_SUCCESS, JSON_Boolean false);
     (STR_PAYLOAD, (JSON_String msg))].
