src/Manifest_JSON_Admits.v
@@ -1,27 +1,27 @@
-Require Import StringT JSON.
+Require Import String JSON.
 
 (* Manifest Admits *)
-Definition MAN_ABS_PLC : StringT. Admitted.
+Definition MAN_ABS_PLC : string. Admitted.
 
-Definition MAN_ASPS : StringT. Admitted.
+Definition MAN_ASPS : string. Admitted.
 
-Definition MAN_APPR_ASPS : StringT. Admitted.
+Definition MAN_APPR_ASPS : string. Admitted.
 
-Definition MAN_UUID_PLCS : StringT. Admitted.
+Definition MAN_UUID_PLCS : string. Admitted.
 
-Definition MAN_PUBKEY_PLCS : StringT. Admitted.
+Definition MAN_PUBKEY_PLCS : string. Admitted.
 
-Definition MAN_TARGET_PLCS : StringT. Admitted.
+Definition MAN_TARGET_PLCS : string. Admitted.
 
-Definition MAN_POLICY : StringT. Admitted.
+Definition MAN_POLICY : string. Admitted.
 
 (* AM Lib Admits *)
-Definition AM_CLONE_UUID : StringT. Admitted.
+Definition AM_CLONE_UUID : string. Admitted.
 
-Definition AM_LIB_ASPS : StringT. Admitted.
+Definition AM_LIB_ASPS : string. Admitted.
 
-Definition AM_LIB_APPR_ASPS : StringT. Admitted.
+Definition AM_LIB_APPR_ASPS : string. Admitted.
 
-Definition AM_LIB_PLCS : StringT. Admitted.
+Definition AM_LIB_PLCS : string. Admitted.
 
-Definition AM_LIB_PUBKEYS : StringT. Admitted.
+Definition AM_LIB_PUBKEYS : string. Admitted.
