src/Term_Defs_Admits.v
@@ -1,22 +1,22 @@
-Require Import Term_Defs_Core Term_Defs ResultT StringT.
+Require Import Term_Defs_Core Term_Defs ResultT String.
 
-Fixpoint Term_to_stringT (t : Term) : StringT. Admitted.
-Definition stringT_to_Term (s : StringT) : ResultT Term StringT. Admitted.
+Fixpoint Term_to_string (t : Term) : string. Admitted.
+Definition string_to_Term (s : string) : ResultT Term string. Admitted.
 
-Definition Evidence_to_stringT (e:Evidence) : StringT. Admitted.
-Definition stringT_to_Evidence (s:StringT) : ResultT Evidence StringT. Admitted.
+Definition Evidence_to_string (e:Evidence) : string. Admitted.
+Definition string_to_Evidence (s:string) : ResultT Evidence string. Admitted.
 
-Fixpoint AppResultC_to_stringT (res: AppResultC) : StringT. Admitted.
-Definition stringT_to_AppResultC (s: StringT) : ResultT AppResultC StringT. Admitted.
+Fixpoint AppResultC_to_string (res: AppResultC) : string. Admitted.
+Definition string_to_AppResultC (s: string) : ResultT AppResultC string. Admitted.
 
-Definition RawEv_to_stringT (e:RawEv) : StringT. Admitted.
-Definition stringT_to_RawEv (s:StringT) : ResultT RawEv StringT. Admitted.
+Definition RawEv_to_string (e:RawEv) : string. Admitted.
+Definition string_to_RawEv (s:string) : ResultT RawEv string. Admitted.
 
-Definition EvC_to_stringT (e:EvC) : StringT. Admitted.
-Definition stringT_to_EvC (s:StringT) : ResultT EvC StringT. Admitted.
+Definition EvC_to_string (e:EvC) : string. Admitted.
+Definition string_to_EvC (s:string) : ResultT EvC string. Admitted.
 
-Fixpoint Ev_to_stringT (e:Ev) : StringT. Admitted.
-Definition stringT_to_Ev (s:StringT) : ResultT Ev StringT. Admitted.
+Fixpoint Ev_to_string (e:Ev) : string. Admitted.
+Definition string_to_Ev (s:string) : ResultT Ev string. Admitted.
 
-Definition ASP_ARGS_to_stringT (args:ASP_ARGS) : StringT. Admitted.
-Definition stringT_to_ASP_ARGS (s:StringT) : ResultT ASP_ARGS StringT. Admitted.
+Definition ASP_ARGS_to_string (args:ASP_ARGS) : string. Admitted.
+Definition string_to_ASP_ARGS (s:string) : ResultT ASP_ARGS string. Admitted.
